pneutube port

test/tube/Hacl.Tube.fst
@@ -10,18 +10,45 @@ open Hacl.Constants
 open Hacl.Cast
 open Box.Ideal
 
+module  U8=FStar.UInt8
+module U32=FStar.UInt32
 module U64=FStar.UInt64
+
+module  H8=Hacl.UInt8
+module H32=Hacl.UInt32
+module H64=Hacl.UInt64
+
 
 #set-options "--lax"
 
+(* JK: Putting here some toplevel constant *)
+inline_for_extraction let blocksize_bits = 18ul
+inline_for_extraction let blocksize = U64 (256uL *^ 1024uL) //1uL <<^ blocksize_bits) // 256 * 1024
+inline_for_extraction let blocksize_32 = U32 (256ul *^ 1024ul) //(1ul <<^ blocksize_bits) // 256 * 1024
+inline_for_extraction let cipherlen (x:U64.t)  = U64 (x +^ 16uL)
+inline_for_extraction let cipherlen_32 (x:U32.t) = U32 (x +^ 16ul)
+inline_for_extraction let ciphersize = cipherlen (blocksize)
+inline_for_extraction let ciphersize_32 = cipherlen_32 (blocksize_32)
+inline_for_extraction let headersize = 1024uL
+inline_for_extraction let headersize_32 = 1024ul
+
+inline_for_extraction let one_64  = Hacl.Cast.uint64_to_sint64 1uL
+inline_for_extraction let zero_64 = Hacl.Cast.uint64_to_sint64 0uL
+inline_for_extraction let one_8  = Hacl.Cast.uint8_to_sint8 1uy
+inline_for_extraction let zero_8 = Hacl.Cast.uint8_to_sint8 0uy
+
+
 type clock = u64
 type str = uint8_p
+
 
 type boxtype =
   | BOX_CHACHA_POLY
   | SECRETBOX_CHACHA_POLY
 
+
 type streamID = b:buffer h8{length b = 16}
+
 
 type open_result = {
   r: FileIO.Types.fresult;
@@ -42,6 +69,7 @@ let opened r fs sid = {r = r; sid = sid; fs = fs}
 
 assume val sent: FStar.HyperStack.mem -> pkA: seq h8 -> pkB: seq h8 -> sid:seq h8 -> FileIO.Types.file_stat -> (seq h8) -> GTot bool
 
+
 val makeStreamID: unit -> StackInline streamID
   (requires (fun h -> True))
   (ensures  (fun h0 r h1 -> True))
@@ -50,10 +78,54 @@ let makeStreamID () =
     randombytes_buf b (U64.uint_to_t 16);
     b
 
-val putU64: z:h64 -> b:uint8_p -> StackInline unit
-  (requires (fun h -> live h b /\ length b = 8))
-  (ensures  (fun h0 r h1 -> live h1 b))
-let putU64 z b =
+
+(* val putU64: z:h64 -> b:uint8_p -> StackInline unit *)
+(*   (requires (fun h -> live h b /\ length b = 8)) *)
+(*   (ensures  (fun h0 r h1 -> live h1 b)) *)
+(* let putU64 z b = *)
+(*   let open Hacl.UInt64 in *)
+(*   b.(0ul) <- sint64_to_sint8 z; *)
+(*   b.(1ul) <- sint64_to_sint8 (z >>^ 8ul); *)
+(*   b.(2ul) <- sint64_to_sint8 (z >>^ 16ul); *)
+(*   b.(3ul) <- sint64_to_sint8 (z >>^ 24ul); *)
+(*   b.(4ul) <- sint64_to_sint8 (z >>^ 32ul); *)
+(*   b.(5ul) <- sint64_to_sint8 (z >>^ 40ul); *)
+(*   b.(6ul) <- sint64_to_sint8 (z >>^ 48ul); *)
+(*   b.(7ul) <- sint64_to_sint8 (z >>^ 56ul) *)
+
+
+(* JK: move to a standard library ? Or use the string library ? *)
+val strlen_: s:str -> len:U32.t ->
+  Stack U32.t
+    (requires (fun h -> live h s)) // Also assumes that the '0uy' will appears somewhere
+    (ensures (fun h0 r h1 -> h0==h1 /\ U32.v r <= length s))
+let rec strlen_ s len =
+  let si = s.(len) in
+  if U8 (si =^ 0uy) then len
+  else strlen_ s (U32 (len +^ 1ul))
+
+val strlen:
+  string:str -> Stack U32.t
+    (requires (fun h -> live h string)) // Also assumes that the '0uy' will appears somewhere
+    (ensures (fun h0 r h1 -> h0==h1 /\ U32.v r <= length string))
+let strlen s = strlen_ s 0ul
+
+type timespec = {
+  tv_sec: U64.t;
+  tv_nsec: U64.t;
+}
+
+
+assume val clock_gettime: unit -> St timespec
+
+
+val store64_le:
+  b:uint8_p{length b = 8} ->
+  z:H64.t ->
+  Stack unit
+    (requires (fun h -> live h b))
+    (ensures  (fun h0 _ h1 -> live h1 b /\ modifies_1 b h0 h1))
+let store64_le b z =
   let open Hacl.UInt64 in
   b.(0ul) <- sint64_to_sint8 z;
   b.(1ul) <- sint64_to_sint8 (z >>^ 8ul);
@@ -64,12 +136,87 @@ let putU64 z b =
   b.(6ul) <- sint64_to_sint8 (z >>^ 48ul);
   b.(7ul) <- sint64_to_sint8 (z >>^ 56ul)
 
-val file_send: file:str -> roundup:u64 ->
-       host:str -> port:u32 ->
-       skA:uint8_p -> pkB:uint8_p ->
-           Stack open_result
-	   (requires (fun _ -> True))
-	   (ensures  (fun h0 s h1 -> match s.r with
+
+val load64_le:
+  b:uint8_p{length b >= 8} ->
+  Stack h64
+    (requires (fun h -> live h b))
+    (ensures  (fun h0 _ h1 -> h0 == h1))
+let load64_le b =
+  let b0 = b.(0ul) in
+  let b1 = b.(1ul) in
+  let b2 = b.(2ul) in
+  let b3 = b.(3ul) in
+  let b4 = b.(4ul) in
+  let b5 = b.(5ul) in
+  let b6 = b.(6ul) in
+  let b7 = b.(7ul) in
+  H64 (
+    sint8_to_sint64 b0
+    |^ (sint8_to_sint64 b1 <<^ 8ul)
+    |^ (sint8_to_sint64 b2 <<^ 16ul)
+    |^ (sint8_to_sint64 b3 <<^ 24ul)
+    |^ (sint8_to_sint64 b4 <<^ 32ul)
+    |^ (sint8_to_sint64 b5 <<^ 40ul)
+    |^ (sint8_to_sint64 b6 <<^ 48ul)
+    |^ (sint8_to_sint64 b7 <<^ 56ul)
+  )
+
+
+
+val file_send_loop:
+  fh:buffer file_handle{length fh = 1} ->
+  sb:buffer socket{length sb = 1} ->
+  ciphertext:uint8_p{Buffer.length ciphertext = U64.v blocksize} ->
+  nonce:uint8_p{Buffer.length nonce = 24} ->
+  key:uint8_p{Buffer.length key = 24} ->
+  seqno:H64.t ->
+  len:U64.t ->
+  Stack sresult
+    (requires (fun h -> live h fh /\ live h sb /\ live h ciphertext /\ live h nonce
+      /\ live h key))
+    (ensures  (fun h0 _ h1 -> True))
+let rec file_send_loop fh sb ciphertext nonce key seqno len =
+  if U64 (len =^ 0uL) then SocketOk
+  else (
+    let i = U64 (len -^ 1uL) in
+    let next = file_next_read_buffer fh blocksize in
+    store64_le (sub nonce 16ul 8ul) seqno;
+    let seqno = H64 (seqno +^ Hacl.Cast.uint64_to_sint64 1uL) in
+    let _ = Hacl.Box.crypto_box_easy_afternm ciphertext next blocksize nonce key in
+    match tcp_write_all sb ciphertext ciphersize with
+    | SocketOk -> file_send_loop fh sb ciphertext nonce key seqno i
+    | SocketError -> SocketError
+  )
+
+
+val file_send_loop_2:
+  fh:buffer file_handle{length fh = 1} ->
+  sb:buffer socket{length sb = 1} ->
+  ciphertext:uint8_p{Buffer.length ciphertext = U64.v blocksize} ->
+  plaintext:uint8_p{Buffer.length plaintext = U64.v blocksize} ->
+  nonce:uint8_p{Buffer.length nonce = 24} ->
+  key:uint8_p{Buffer.length key = 24} ->
+  len:U64.t ->
+  St sresult
+let rec file_send_loop_2 fh sb ciphertext plaintext nonce key len =
+  if U64 (len =^ 0uL) then SocketOk
+  else (
+    let i = U64 (len -^ 1uL) in
+    let _ = Hacl.Box.crypto_box_easy_afternm ciphertext plaintext blocksize nonce key in
+    match tcp_write_all sb ciphertext ciphersize with
+    | SocketOk -> file_send_loop_2 fh sb ciphertext plaintext nonce key i
+    | SocketError -> SocketError
+  )
+
+
+val file_send:
+  file:str -> roundup:u64 ->
+  host:str -> port:u32 ->
+  skA:uint8_p -> pkB:uint8_p ->
+  Stack open_result
+    (requires (fun _ -> True))
+    (ensures  (fun h0 s h1 -> match s.r with
       	   	                   | FileOk ->
 				     let fs = s.fs in
 				     let sidb = s.sid in
@@ -81,30 +228,294 @@ val file_send: file:str -> roundup:u64 ->
 				   | _ -> true))
 let file_send f r h p skA pkB =
   push_frame();
-  let sid = makeStreamID() in
+  (* Initializing all buffers on the stack *)
+  let pkA = Buffer.create (Hacl.Cast.uint8_to_sint8 0uy) 32ul in
+  let zero = Hacl.Cast.uint8_to_sint8 0uy in
+  let nine = Hacl.Cast.uint8_to_sint8 9uy in
+  let basepoint = Buffer.createL [
+    nine; zero; zero; zero; zero; zero; zero; zero; zero; zero; zero; zero; zero; zero; zero; zero;
+    zero; zero; zero; zero; zero; zero; zero; zero; zero; zero; zero; zero; zero; zero; zero; zero
+  ] in
+  Hacl.EC.Curve25519.exp pkA basepoint skA;
+
+  (* Initialization of the file_handle *)
   let dummy_ptr = FStar.Buffer.create (Hacl.Cast.uint8_to_sint8 0uy) 1ul in
-  let fh = init_file_handle(dummy_ptr) in
-  let fb = Buffer.create fh 1ul in
+  let fb = Buffer.create (init_file_handle(dummy_ptr)) 1ul in
+
+  (* Initialization of the sessionID *)
+  let sid = makeStreamID() in
+
   let res =
     match (file_open_read_sequential f fb) with
     | FileOk ->
+        (* Read file handle value *)
         let fh = fb.(0ul) in
+        (* Initialization of the socket *)
         let s = init_socket() in
         let sb = Buffer.create s 1ul in
         (match tcp_connect h p sb with
         | SocketOk ->
-	    (* let s = sb.(0ul) in *)
-	    (match tcp_write_all sb sid 8uL with
-	    | SocketOk -> opened FileOk fh.stat sid
-	    | SocketError -> opened FileError fh.stat sid)
-        | SocketError -> opened FileError fh.stat sid)
-    | FileError -> opened FileError fh.stat sid in
+	    let s = sb.(0ul) in
+            let ciphertext = Buffer.create zero ciphersize_32 in
+            let file_size = fh.stat.size in
+            (* JK: I assume that blocksize is a power of 2 *)
+            let fragments = H64 (file_size >>^ blocksize_bits) in
+            let rem = H64 (file_size &^ (blocksize-^one_64)) in
+            let roundup = Hacl.Cast.uint64_to_sint64 r in
+            (* JK: I assume that roundup is a power of 2, otherwise that is wrong *)
+            let hsize_mod_roundup = H64 (file_size &^ (roundup-^one_64)) in
+            let mask = H64 (gte_mask roundup one_64 &^ (lognot (eq_mask hsize_mod_roundup zero_64))) in
+            let hrem = H64 (roundup -^ hsize_mod_roundup) in
+            let hsize = H64 (file_size -^ hrem) in
+            let mtime = fh.stat.mtime in
+            let nsize = strlen f in
+            let zero_8 = Hacl.Cast.uint8_to_sint8 0uy in
+            let header = Buffer.create zero_8 headersize_32 in
+            (* JK: Omitting memset to 0 for now *)
+            store64_le (Buffer.sub header  0ul 8ul) file_size;
+            store64_le (Buffer.sub header  8ul 8ul) mtime;
+            store64_le (Buffer.sub header 16ul 8ul) (Int.Cast.uint32_to_uint64 nsize);
+            (* JK: Ignoring the test on the file name length for convenience *)
+            Buffer.blit f 0ul header 24ul nsize;
+            (* A buffer to store uint64 values before flushing them *)
+            let buf = Buffer.create zero 8ul in
+            (* Flush the streamID *)
+	    (match tcp_write_all sb sid 16uL with
+	    | SocketOk -> (
+                store64_le buf hsize;
+                match tcp_write_all sb buf 8uL with
+                | SocketOk -> (
+                    match tcp_write_all sb pkA 32uL with
+                    | SocketOk -> (
+                        match tcp_write_all sb pkB 32uL with
+                        | SocketOk -> (
+                            let seqno = Hacl.Cast.uint64_to_sint64 0uL in
+                            let nonce = Buffer.create zero 24ul in
+                            let key   = Buffer.create zero 32ul in
+                            if Hacl.Box.crypto_box_beforenm key pkB pkA = 0ul then (
+                              (* Populating the nonce *)
+                              blit sid 0ul nonce 0ul 16ul;
+                              store64_le (sub nonce 16ul 8ul) seqno;
+                              let seqno = H64 (seqno +^ one_64) in
+                              let _ = Hacl.Box.crypto_box_easy_afternm ciphertext header headersize
+                                                               nonce key in
+                              (match tcp_write_all sb ciphertext (cipherlen headersize) with
+                              | SocketOk -> (
+                                  (* JK: need to declassify fragmensts *)
+                                  match file_send_loop fb sb ciphertext nonce key seqno fragments with
+                                  | SocketOk -> (
+                                      let plaintext = Buffer.create zero blocksize_32 in
+                                      (* JK: Omitting memset to 0 for now *)
+                                      // JK: TODO:hrem and rem are secret, need declassification
+                                      let rem_dec = rem in
+                                      let hrem_dec = hrem in
+                                      if U64 (rem_dec +^ hrem_dec >^ zero_64) then (
+                                        let next = file_next_read_buffer fb rem in
+                                        blit next 0ul plaintext 0ul (Int.Cast.uint64_to_uint32 rem);
+                                        // Here seqno is 1 (header) + fragments (loop) + 1 (here)
+                                        let seqno = (H64 (fragments +^ 2uL)) in
+                                        store64_le (sub nonce 16ul 8ul) seqno;
+                                        let seqno = H64 (seqno +^ one_64) in
+                                        let cond = U64 (rem_dec +^ hrem_dec >^ blocksize) in
+                                        let rem = if cond then blocksize else H64 (rem +^ hrem) in
+                                        let hrem = if cond then H64 (hrem -^ (blocksize -^ rem)) else zero_64 in
+                                        let _ = Hacl.Box.crypto_box_easy_afternm ciphertext plaintext rem nonce key in
+                                        (match tcp_write_all sb ciphertext (cipherlen rem) with
+                                        | SocketOk -> (
+                                            if U64 (hrem >^ 0uL) then (
+                                              Buffer.fill plaintext zero blocksize_32;
+                                              let fragments = U64 (hrem >>^ blocksize_bits) in
+                                              let hrem = U64 (hrem &^ (blocksize -^ one_64)) in
+                                              (match file_send_loop_2 fb sb ciphertext plaintext nonce key fragments with
+                                              | SocketOk ->
+                                                  if U64 (hrem >^ 0uL) then (
+                                                    let _ = Hacl.Box.crypto_box_easy_afternm ciphertext plaintext hrem nonce key in
+                                                    match tcp_write_all sb ciphertext (cipherlen hrem) with
+                                                    | SocketOk -> opened FileOk fh.stat sid
+                                                    | SocketError -> opened FileError fh.stat sid
+                                                  ) else (
+                                                    opened FileOk fh.stat sid
+                                                  )
+                                               | SocketError -> opened FileError fh.stat sid)
+                                            ) else (
+                                              opened FileOk fh.stat sid
+                                            ) )
+                                        | SocketError -> opened FileError fh.stat sid)
+                                      ) else (
+                                        opened FileOk fh.stat sid
+                                      ) )
+                                  | SocketError -> opened FileError fh.stat sid )
+                              | SocketError -> opened FileError fh.stat sid )
+                            ) else (
+                              opened FileOk fh.stat sid
+                            ) )
+                        | SocketError -> opened FileError fh.stat sid )
+                    | SocketError -> opened FileError fh.stat sid )
+                | SocketError -> opened FileError fh.stat sid )
+            | SocketError -> opened FileError fh.stat sid ) )
+    | FileError -> opened FileError (fb.(0ul)).stat sid in
   pop_frame();
   res
 
 
+val memcmp_ct_:
+  b:uint8_p ->
+  b':uint8_p ->
+  len:U32.t ->
+  tmp:H8.t ->
+  Stack U8.t
+    (requires (fun _ -> True))
+    (ensures  (fun _ _ _ -> True))
+let rec memcmp_ct_ b b' len tmp =
+  if U32 (len =^ 0ul) then (
+    (* JK: Declassification needed *)
+    tmp
+  ) else (
+    let i = U32 (len -^ 1ul) in
+    let bi = b.(i) in let bi' = b'.(i) in
+    let tmp = U8 (tmp &^ (eq_mask bi bi')) in
+    memcmp_ct_ b b' i tmp
+  )
+
+(** Constant time comparison function
+    Return 0xff if b == b', 0 otherwise **)
+val memcmp_ct:
+  b:uint8_p ->
+  b':uint8_p ->
+  len:U32.t ->
+  Stack U8.t
+    (requires (fun _ -> True))
+    (ensures  (fun _ _ _ -> True))
+let memcmp_ct b b' len =
+  memcmp_ct_ b b' len (Hacl.Cast.uint8_to_sint8 0xffuy)
+
+
 val get_fh_stat: file_handle -> Tot file_stat
 let get_fh_stat fh = fh.stat
+
+val file_recv_loop_2:
+  fb:buffer file_handle ->
+  connb:buffer socket ->
+  ciphertext:uint8_p ->
+  nonce:uint8_p ->
+  key:uint8_p ->
+  seqno:H64.t ->
+  len:U64.t ->
+  Stack sresult
+    (requires (fun _ -> True))
+    (ensures  (fun _ _ _ -> True))
+let rec file_recv_loop_2 fb connb ciphertext nonce key seqno len =
+  if U64 (len =^ 0uL) then SocketOk
+  else (
+    let i = U64 (len -^ 1uL) in
+    match tcp_read_all connb ciphertext ciphersize with
+    | SocketOk -> (
+        let next = file_next_write_buffer fb blocksize in
+        store64_le nonce seqno;
+        let seqno = H64 (seqno +^ one_64) in
+        if U32 (Hacl.Box.crypto_box_open_easy_afternm next ciphertext ciphersize nonce key =^ 0ul) then
+          file_recv_loop_2 fb connb ciphertext nonce key seqno i
+        (* JK: not distinguishing between socket error and decryption failure *)
+        else SocketError)
+    | SocketError -> SocketError
+  )
+
+
+val file_recv_loop:
+  fb:buffer file_handle ->
+  connb:buffer socket ->
+  lhb:buffer socket ->
+  sid:uint8_p ->
+  pkA:uint8_p ->
+  pkB:uint8_p ->
+  skB:uint8_p ->
+  Stack sresult
+    (requires (fun h -> True))
+    (ensures  (fun h0 _ h1 -> True))
+let rec file_recv_loop fb connb lhb sid pkA pkB skB =
+  push_frame();
+  let res =
+  match tcp_accept lhb connb with
+  | SocketOk -> (
+      let ciphertext = create zero_8 ciphersize_32 in
+      let pk1 = create zero_8 32ul in
+      let pk2 = create zero_8 32ul in
+      let nonce = create zero_8 24ul in
+      (match tcp_read_all connb (sub nonce 0ul 16ul) 16uL with
+      | SocketOk -> (
+          (* JK: no check on the streamID formatting *)
+          match tcp_read_all connb (sub nonce 16ul 8ul) 8uL with
+          | SocketOk -> (
+              (* JK: no check on the size *)
+              match tcp_read_all connb pk1 32uL with
+              | SocketOk -> (
+                  match tcp_read_all connb pk2 32uL with
+                  | SocketOk -> (
+                      if U8 (memcmp_ct pk1 pkA 32ul =^ 0xffuy) then (
+                         if U8 (memcmp_ct pk2 pkB 32ul =^ 0xffuy) then (
+                           let key = create zero_8 32ul in
+                           (* JK: ignoring check on beforenm *)
+                           let _ = Hacl.Box.crypto_box_beforenm key pkA pkB in
+                           let seqno = 0uL in
+                           let header = create zero_8 headersize_32 in
+                           fill header zero_8 headersize_32;
+                           (match tcp_read_all connb ciphertext (cipherlen(headersize)) with
+                           | SocketOk -> (
+                               store64_le (sub nonce 16ul 8ul) seqno;
+                               let seqno = H64 (seqno +^ 1uL) in
+                               if U32 (Hacl.Box.crypto_box_open_easy_afternm header ciphertext (cipherlen(headersize)) nonce key =^ 0ul) then (
+                                 let file_size = load64_le (sub header 0ul  8ul) in
+                                 let nsize     = load64_le (sub header 8ul  8ul) in
+                                 let mtime     = load64_le (sub header 16ul 8ul) in
+                                 (* JK: no checking the size of the filename *)
+                                 (* JK: need declassification on nsize value *)
+                                 let file = sub header 24ul (Int.Cast.uint64_to_uint32 nsize) in
+                                 let fstat = {name = file; mtime = mtime; size = nsize} in
+                                 (match file_open_write_sequential fstat fb with
+                                 | FileOk -> (
+                                     let fragments = H64 (file_size >>^ blocksize_bits) in
+                                     let rem       = H64 (file_size &^ (blocksize -^ one_64)) in
+                                     (match file_recv_loop_2 fb connb ciphertext nonce key seqno fragments with
+                                     | SocketOk -> (
+                                         let res =
+                                           if U64 (rem >^ 0uL) then (
+                                             match tcp_read_all connb ciphertext (cipherlen(rem)) with
+                                             | SocketOk -> (
+                                                 let next = file_next_write_buffer fb rem in
+                                                 let seqno = U64 (fragments +^ 2uL) in
+                                                 if U32 (Hacl.Box.crypto_box_easy_afternm next ciphertext (cipherlen(rem)) nonce key =^ 0ul) then SocketOk
+                                                 else SocketError )
+                                             | SocketError -> SocketError
+                                           ) else SocketOk in
+                                         match res with
+                                         | SocketOk -> (
+                                             match file_close fb with
+                                             | true -> (
+                                                 match tcp_close connb with
+                                                 | SocketOk -> SocketOk
+                                                 | SocketError -> SocketError )
+                                             | false -> SocketError )
+                                         | SocketError -> SocketError )
+                                     | SocketError -> SocketError ) )
+                                 | FileError -> SocketError )
+                               ) else (
+                                 SocketError ) )
+                           | SocketError -> SocketError )
+                         ) else (
+                           SocketError
+                         )
+                       ) else (
+                         SocketError ) )
+                  | SocketError -> SocketError )
+              | SocketError -> SocketError )
+          | SocketError -> SocketError )
+      | SocketError -> SocketError ) )
+  | SocketError -> SocketError in
+  pop_frame();
+  match res with
+  | SocketOk -> file_recv_loop  fb connb lhb sid pkA pkB skB
+  | SocketError -> SocketError
+
 
 val file_recv: port:u32 -> pkA:uint8_p -> skB:uint8_p -> Stack open_result
        	   (requires (fun _ -> True))
@@ -119,10 +530,29 @@ val file_recv: port:u32 -> pkA:uint8_p -> skB:uint8_p -> Stack open_result
 				   | _ -> true))
 let file_recv p pkA skB =
   push_frame();
+  (* Initialization of the file_handle *)
   let dummy_ptr = FStar.Buffer.create (Hacl.Cast.uint8_to_sint8 0uy) 1ul in
-  let sid = makeStreamID() in
   let fh = init_file_handle(dummy_ptr) in
+  let fb = create fh 1ul in
+  let sid = makeStreamID() in
   let stat = get_fh_stat fh in
-  let res = opened FileError stat sid in
+  (* Initialization of the two sockets *)
+  let s = init_socket() in
+  let connb = Buffer.create s 1ul in
+  let lhb = Buffer.create s 1ul in
+  let res = (match tcp_listen p lhb with
+  | SocketOk -> (
+      let pkB = create zero_8 32ul in
+      let zero = zero_8 in
+      let nine = Hacl.Cast.uint8_to_sint8 9uy in
+      let basepoint = Buffer.createL [
+        nine; zero; zero; zero; zero; zero; zero; zero; zero; zero; zero; zero; zero; zero; zero; zero;
+        zero; zero; zero; zero; zero; zero; zero; zero; zero; zero; zero; zero; zero; zero; zero; zero
+      ] in
+      Hacl.EC.Curve25519.exp pkB basepoint skB;
+      match file_recv_loop fb connb lhb sid pkA pkB skB with
+      | SocketOk -> opened FileOk fh.stat sid
+      | SocketError -> opened FileError fh.stat sid )
+  | SocketError -> opened FileError fh.stat sid ) in
   pop_frame();
   res
